\documentclass[11pt,pra,aps]{revtex4}
\usepackage[dvipdfmx]{graphicx}
\usepackage{float}
\usepackage{rotating}
\usepackage{array}
\usepackage{amsmath}
\usepackage{multirow}
\usepackage{setspace}
\usepackage{braket}
\usepackage{epstopdf}
\usepackage{moreverb}
\usepackage{wrapfig}
\usepackage{longtable}

\usepackage{color}                            

\usepackage[dvipdfmx]{hyperref}
\usepackage{pxjahyper}

\newcommand{\red}[1]{\textcolor{red}{#1}}     
\newcommand{\blue}[1]{\textcolor{blue}{#1}}

\newcommand{\boxz}[1]{\boxed{\red{\text{#1}}}}
%\newcommand{\boxz}[1]{\boxed{\phantom{\text{#1}}}}
\newcommand{\boxa}[1]{\boxed{\phantom{}}}

%%\renewcommand{\baselinestretch}{2.0}

\renewcommand{\thefigure}{S\arabic{figure}}
\renewcommand{\thetable}{S\arabic{table}}

\begin{document}
    
\begin{align}
  E_\text{trial}(\alpha;r)=\frac{\langle \psi_\text{trial}|H|\psi_\text{trial}\rangle}{\langle \psi_\text{trial}|\psi_\text{trial}\rangle}
\end{align}

\begin{align}
  \int^\infty_0 x^{2n}e^{-ax^2}dx&=\frac{1\cdot3\cdot5\cdots(2n-1)}{2^{2n+1}a^n}\sqrt{\frac{\pi}{a}} \\
  \int^\infty_0 x^{2n+1}e^{-ax^2}dx&=\frac{n!}{2a^{n+1}}
\end{align}

\begin{align}
  \langle \psi_\text{trial}|\psi_\text{trial}\rangle &= \int^{2\pi}_0d\phi\int^{\pi}_{0}d\theta\sin\theta\int^{\infty}_{0} dr\ r^2 e^{-2\alpha r^2} \\
  &= 4\pi\int^{\infty}_{0} dr\ r^2 e^{-2\alpha r^2} \\
  &= \frac{4\pi }{8\alpha}\sqrt{\frac{\pi}{2\alpha}}
\end{align}

\begin{align}
  \langle \psi_\text{trial}|H|\psi_\text{trial}\rangle &= 4\pi\int^{\infty}_{0} dr\ r^2 e^{-\alpha r^2}\ \left[-\frac{\hbar^2}{2m_e r^2}\frac{d}{dr}\left(r^2\frac{d}{dr}\right)-\frac{e^2}{4\pi\epsilon_0 r}\right]\ e^{-\alpha r^2}\\
  &= 4\pi\int^{\infty}_{0} dr\ r^2 e^{-\alpha r^2}\ \left[-\frac{\hbar^2}{2m_e r^2}(-6\alpha r^2+4\alpha^2r^4)-\frac{e^2}{4\pi\epsilon_0 r}\right]\ e^{-\alpha r^2}\\
  &= 4\pi\left[ \frac{3\hbar^2}{8m_e} \sqrt{\frac{\pi}{2\alpha}}  - \frac{3\hbar^2}{16m_e} \sqrt{\frac{\pi}{2\alpha}} - \frac{e^2}{16\pi\epsilon_0}\cdot\frac{1}{\alpha} \right] \\
  &= 4\pi\left[ \frac{3\hbar^2}{16m_e} \sqrt{\frac{\pi}{2\alpha}}  - \frac{e^2}{16\pi\epsilon_0}\cdot\frac{1}{\alpha} \right]  
\end{align}

\begin{align}
  E_\text{trial}(\alpha)=\frac{3\hbar^2}{2m_e}\alpha - \frac{e^2}{2\pi\epsilon_0}\sqrt{\frac{2\alpha}{\pi}}
\end{align}

\begin{align}
  \frac{\partial E_\text{trial}(\alpha)}{\partial \alpha}&=\frac{3\hbar^2}{2m_e} - \frac{e^2}{4\pi\epsilon_0}\sqrt{\frac{2}{\pi\alpha}}\rightarrow 0 \\
  &\Rightarrow \alpha_\text{min} = \frac{m_e^2 e^4}{18\pi^3 \hbar^4 \epsilon_0^2}
\end{align}

\begin{align}
  E_\text{trial}(\alpha_\text{min})&=-\frac{m_e e^4}{12 \pi^3 \epsilon_0 \hbar^2} \\
  &=-\frac{4}{3\pi}\left(\frac{m_e e^4}{16 \pi^2 \epsilon_0 \hbar^2}\right) \\
  &=-\frac{4}{3\pi}\ \text{Eh} = \red{0.424\ \text{Eh}}  
\end{align}

\begin{align}
  H=-\frac{\hbar^2}{2\mu r^2}\frac{d}{dr}\left(r^2\frac{d}{dr}\right)+\frac{k}{2}r^2
\end{align}

\begin{align}
  H=-\frac{\hbar^2}{2\mu}\nabla^2+\frac{k}{2}\left(x^2+y^2+z^2\right)
\end{align}

\begin{align}
  E_\text{ground state}=\frac{3}{2}\hbar\omega
\end{align}

\begin{align}
  \langle \psi_\text{trial}|H|\psi_\text{trial}\rangle &= 4\pi\int^{\infty}_{0} dr\ r^2 e^{-\alpha r^2}\ \left[-\frac{\hbar^2}{2\mu r^2}\frac{d}{dr}\left(r^2\frac{d}{dr}\right)+\frac{k}{2}r^2\right]\ e^{-\alpha r^2}\\
  &= 4\pi\left[ \frac{3\hbar^2}{16\mu} \sqrt{\frac{\pi}{2\alpha}}  - \frac{k}{2}\frac{3}{32\alpha^2} \sqrt{\frac{\pi}{2\alpha}} \right]
\end{align}

\begin{align}
  E_\text{trial}(\alpha)=\frac{3\hbar^2}{2\mu}\alpha + \frac{3k}{8\alpha}
\end{align}

\begin{align}
  \frac{\partial E_\text{trial}(\alpha)}{\partial \alpha}&=\frac{3\hbar^2}{2\mu} - \frac{3k}{8\alpha}\rightarrow 0 \\
  &\Rightarrow \alpha_\text{min} = \frac{\sqrt{\mu k}}{2\hbar}
\end{align}

\begin{align}
  E_\text{trial}(\alpha_\text{min})=\frac{3}{2}\hbar\sqrt{\frac{k}{\mu}}=\red{\frac{3}{2}\hbar\omega}
\end{align}

\begin{align}
  \psi_\text{trial}(\alpha;r)=N\exp\left(-\alpha r\right)
\end{align}

\begin{align}
  \langle \psi_\text{trial}|H|\psi_\text{trial}\rangle &= 4\pi\int^{\infty}_{0} dr\ r^2 e^{-\alpha r}\ \left[-\frac{\hbar^2}{2\mu r^2}\frac{d}{dr}\left(r^2\frac{d}{dr}\right)+\frac{k}{2}r^2\right]\ e^{-\alpha r}\\
  &= 4\pi\left[ -\frac{\hbar^2}{2\mu}\left(\frac{1}{4\alpha}-\frac{1}{2\alpha}\right) + \frac{k}{2}\left(\frac{3}{4\alpha^5}\right)\right]
\end{align}

\begin{align}
  \langle \psi_\text{trial}|\psi_\text{trial}\rangle = 4\pi\int^{\infty}_{0} dr\ r^2 e^{-2\alpha r}=4\pi \frac{1}{4\alpha^3}
\end{align}

\begin{align}
  E_\text{trial}(\alpha)=\frac{\hbar^2\alpha^2}{2\mu}+\frac{3k}{2\alpha^2}
\end{align}

\begin{align}
  \frac{\partial E_\text{trial}(\alpha)}{\partial \alpha}&=\frac{2\hbar^2\alpha}{2\mu} - \frac{3k}{\alpha^3}\rightarrow 0 \\
  &\Rightarrow \alpha_\text{min} = \left(\frac{3 \mu k}{\hbar^2}\right)^{1/4}
\end{align}

\begin{align}
  E_\text{trial}(\alpha_\text{min})=\sqrt{3}\hbar\sqrt{\frac{k}{\mu}}={\sqrt{3}\hbar\omega}=\red{1.7321\hbar\omega>E_\text{ground state}}
\end{align}

\begin{align}
  [x,p]&=i\hbar\left(-x\frac{\partial}{\partial x}+\frac{\partial}{\partial x}x\right) \\
  &=i\hbar\left(-x\frac{\partial}{\partial x}+1+x\frac{\partial}{\partial x}\right) \\
  &=i\hbar
\end{align}

\begin{align}
  \langle\psi|[x,p]|\psi\rangle &= i\hbar\int_A dx\ \psi^{*}\psi = i\hbar
\end{align}

\begin{align}
  \langle\psi|[L_z,\phi]|\psi\rangle &= -i\hbar\int^{2\pi}_0 d\phi\ \psi^{*}(\phi)\ \psi(\phi) = -i\hbar
\end{align}

\begin{align}
  \langle\phi\rangle=\frac{\int^{2\pi}_0 \phi\ 1^2\ d\phi}{\int^{2\pi}_0 1^2\ d\phi}=\frac{\frac{1}{2}[\phi^2]^{2\pi}_0}{[\phi]^{2\pi}_0}=\pi
\end{align}

\begin{align}
  \Delta\phi = \sqrt{\langle\phi^2\rangle-\langle\phi\rangle^2}=\frac{\pi}{\sqrt{3}}
\end{align}

\begin{align}
  \int^{2\pi}_0 \left[(L_z\psi)^{*}(\phi\psi)-(\phi\psi)^{*}(L_z\psi)\right]d\phi
\end{align}

\begin{align}
  \int^{2\pi}_0 (L_z\psi)^{*}(\phi\psi)d\phi &= \int^{2\pi}_0 \left(-i\hbar\frac{\partial}{\partial \phi}\psi\right)^{*}(\phi\psi)d\phi \\
  &= i\hbar \int^{2\pi}_0 \left(\frac{\partial \psi^{*}}{\partial \phi}\right)(\phi\psi)d\phi \\
  &= i\hbar \left\{[\phi|\psi|^2]^{2\pi}_0-\int^{2\pi}_0 \left(|\psi|^2+\phi\psi^{*}\frac{\partial\psi}{\partial\phi}\right) d\phi \right\}\\
  &= i\hbar \left\{2\pi|\psi(2\pi)|^2-1-\int^{2\pi}_0 \phi\psi^{*}\frac{\partial\psi}{\partial\phi} d\phi \right\}\\
\end{align}

\begin{align}
  \int^{2\pi}_0 (\phi\psi)^{*}(L_z\psi)d\phi &= \int^{2\pi}_0 (\phi\psi)^{*} \left(-i\hbar\frac{\partial}{\partial \phi}\psi\right)d\phi \\
  &= -i\hbar \int^{2\pi}_0 \phi\psi^{*} \frac{\partial \psi}{\partial \phi} d\phi \\
\end{align}

\begin{align}
  \int^{2\pi}_0 \left[(L_z\psi)^{*}(\phi\psi)-(\phi\psi)^{*}(L_z\psi)\right]d\phi = i\hbar \left\{2\pi|\psi(2\pi)|^2-1 \right\}
\end{align}

\begin{align}
  \Delta L_z \Delta \phi \geq \frac{\hbar}{2} \left|1-2\pi|\psi(2\pi)|^2\right|
\end{align}

\begin{align}
  \frac{\partial}{\partial \xi} &= \frac{\partial}{\partial x}\frac{\partial x}{\partial \xi}=\frac{1}{a}\frac{\partial}{\partial x} \\
  \frac{\partial^2}{\partial \xi^2} &=\frac{1}{a^2}\frac{\partial^2}{\partial x^2} = \sqrt{\frac{\hbar}{m\omega}}\frac{\partial^2}{\partial x^2}\\  
\end{align}

\begin{align}
  -\frac{\hbar}{2m}\frac{m\omega}{\hbar}\frac{\partial^2\psi}{\partial \xi^2}+\frac{1}{2}m\omega^2\frac{\hbar}{m\omega}\xi^2\psi=E\psi
\end{align}

\begin{align}
  -\frac{\partial^2\psi}{\partial \xi^2}+\xi^2\psi=\frac{2E}{m\omega}\psi=\epsilon\psi
\end{align}

\begin{align}
  \left[-\frac{\hbar\omega}{2}\frac{\partial^2}{\partial \xi^2}+\frac{\hbar\omega}{2}\xi^2+A\cdot\frac{2}{\hbar\omega}\cdot\left(\frac{\hbar}{m\omega}\right)^2\xi^4\right]\psi=E\psi
\end{align}

\begin{align}
  \left[-\frac{\partial^2}{\partial \xi^2}+\xi^2+\lambda\xi^4\right]\psi=\epsilon\psi
\end{align}

\begin{align}
\lambda=\frac{2\hbar A}{m^2\omega^3}
\end{align}

\begin{align}
  \int^{\infty}_{-\infty}x^{2n}e^{-ax^2}\ dx = \frac{1\cdot3\cdot5\cdots(2n-1)}{2^n a^n}\sqrt{\frac{\pi}{a}}
\end{align}

\begin{align}
  \epsilon^{(1)}_0&=\int^{\infty}_{-\infty} \psi^{(0)}_0\left(\lambda \xi^4\right) \psi^{(0)}_0 d\xi \\
  &=\frac{\lambda}{\sqrt{\pi}} \int^{\infty}_{-\infty} \xi^4 e^{-\xi^2} d\xi=\frac{3}{4}\frac{\lambda}{\pi}\cdot\sqrt{\pi}=\frac{3}{4}\lambda=0.75\lambda
\end{align}

\begin{align}
  \epsilon^{(1)}_1&=\int^{\infty}_{-\infty} \psi^{(0)}_1\left(\lambda \xi^4\right) \psi^{(0)}_1 d\xi \\
  &= \frac{2\lambda}{\sqrt{\pi}} \int^{\infty}_{-\infty} \xi^6 e^{-\xi^2} d\xi = \frac{2\lambda}{\sqrt{\pi}}\cdot\frac{15}{8}\sqrt{\pi} = \frac{15}{4}\lambda=3.75\lambda
\end{align}

\begin{align}
  \epsilon^{(1)}_2&=\int^{\infty}_{-\infty} \psi^{(0)}_2\left(\lambda \xi^4\right) \psi^{(0)}_2 d\xi \\
  &= \frac{\lambda}{8\sqrt{\pi}} \int^{\infty}_{-\infty} \xi^4 (4\xi^2-2)^2 e^{-\xi^2} d\xi \\
  &= \frac{\lambda}{8\sqrt{\pi}} \int^{\infty}_{-\infty} \xi^4 (16\xi^4-16\xi^2+4) e^{-\xi^2} d\xi \\
  &= \frac{\lambda}{8\sqrt{\pi}} \left(16\cdot\frac{3\cdot5\cdot7}{2^4}-16\cdot\frac{3\cdot5}{2^3}+4\cdot\frac{3}{2^2}\right) \sqrt{\pi}\\
  &= \frac{\lambda}{8\sqrt{\pi}} \left(105-30+3\right) \sqrt{\pi}=\frac{39}{4}\lambda=9.75\lambda\\
\end{align}

\end{document}
